Replace PSField with more methods in CrVarLike typeclass.
Rationale: Avoid duplicate mechanisms (PSField and CrVarLike) for same goal (unify Header, State, Ctrl).

Also use Ltac to avoid redundant proofs.

CrVarLike.v
@@ -3,6 +3,10 @@ From MyProject Require Import Integers.
 From MyProject Require Import MyInts.
 From MyProject Require Import InitStatus.
 From MyProject Require Import CrIdentifiers.
+From MyProject Require Import CrProgramState.
+From MyProject Require Import SmtExpr.
+From MyProject Require Import CrDsl.
+From MyProject Require Import Maps.
 Require Import ZArith.
 Require Import Bool.
 Require Import List.
@@ -11,12 +15,52 @@ Import ListNotations.
 Definition injective_contravariant {A B} (f : A -> B) : Prop :=
   forall x y, x <> y -> f x <> f y.
 
+Definition program_state_mapper {T1 T2 : Type} (fc: T1 -> T2) (fh : T1 -> T2) (fs : T1 -> T2) (s: ProgramState T1) : ProgramState T2 :=
+  {| ctrl_map := PMap.map fc (ctrl_map s);
+     header_map := PMap.map fh (header_map s);
+     state_map := PMap.map fs (state_map s) |}.
+
 Class CrVarLike (A : Type) := {
   make_item : positive -> A;
   get_key   : A -> positive;
+  map_from_ps : forall {T}, (ProgramState T) -> PMap.t T;
+  lookup_varlike_map : forall {T}, PMap.t T -> A -> T := fun {T} m x => PMap.get (get_key x) m;
+  lookup_varlike : forall {T}, (ProgramState T) -> A -> T := fun {T} s x => lookup_varlike_map (map_from_ps s) x;
+  update_all_varlike : forall {T}, (ProgramState T) -> (A -> T) -> ProgramState T;
+  update_varlike : forall {T}, (ProgramState T) -> A -> T -> ProgramState T;
+  is_varlike_in_ps : forall {T}, (ProgramState T) -> A -> option T := fun {T} s v => PTree.get (get_key v) (snd (map_from_ps s));
+
+  (* Simple Lemmas *)
   inverses : forall (x : A), make_item (get_key x) = x;
   inverses' : forall (i : positive), get_key (make_item i) = i;
   inj : injective_contravariant get_key;
+
+  (* Harder lemmas *)
+  update_all_varlike_lookup_unchanged :
+  forall {T} (s1 : ProgramState T),
+  update_all_varlike s1 (fun v : A => lookup_varlike_map (map_from_ps s1) v) = s1;
+
+  commute_lookup_varlike:
+  forall {T1 T2} ps v (func : T1 -> T2),
+  lookup_varlike (program_state_mapper func func func ps) v = func (lookup_varlike_map (map_from_ps ps) v);
+
+  commute_mapper_update_varlike:
+  forall {T1 T2} ps x v (func : T1 -> T2),
+  program_state_mapper func func func (update_varlike ps x v) = update_varlike (program_state_mapper func func func ps) x (func v);
+
+  lookup_varlike_after_update_all_varlike:
+  forall {T} (s1 : ProgramState T) (v : A) (fv : A -> T),
+    is_varlike_in_ps s1 v <> None ->
+    lookup_varlike_map (map_from_ps (update_all_varlike s1 fv)) v = fv v;
+}.
+
+Class CrVarLikePairLemmas (A A' : Type) `(CrVarLike A) `(CrVarLike A') := {
+  test : A; (*TODO: doesn't compile without this. FIX *)
+  commute_varlike_updates:
+  forall {T} (s1 : ProgramState T)
+    (fv : A -> T) (fv' : A' -> T),
+    update_all_varlike (update_all_varlike s1 fv') fv =
+    update_all_varlike (update_all_varlike s1 fv) fv';
 }.
 
 Ltac prove_inj :=
@@ -25,40 +69,142 @@ Ltac prove_inj :=
   rewrite Heq in Hxy;
   congruence.
 
+(* Function to go through all keys in a PMap, and set them to new values. *)
+Definition new_pmap_from_old {T: Type} (old_pmap : PMap.t T) (f : positive -> T): PMap.t T :=
+  (fst old_pmap, (* The old default value *)
+   PTree.map (fun x _ => f x) (snd old_pmap) (* Take old tree (snd old_pmap) and map elements from it (x) via function (f) *)
+  ).
+
+Ltac prove_update_all_varlike_lookup_unchanged arg :=
+  intros T s1;
+  destruct s1 as [ctrl hdr state];
+  unfold new_pmap_from_old;
+  destruct arg as [t t0]; simpl;
+  f_equal; f_equal;
+  apply PTree.extensionality;
+  intros i;
+  rewrite PTree.gmap;
+  destruct (t0 ! i) eqn:des; auto;
+  simpl;
+  unfold PMap.get;
+  simpl;
+  rewrite des;
+  reflexivity.
+
+Ltac prove_commute_mapper_update_varlike :=
+  intros T1 T2 ps x v func;
+  destruct ps;
+  unfold program_state_mapper;
+  f_equal;
+  simpl;
+  unfold PMap.set;
+  unfold PMap.map;
+  simpl;
+  f_equal;
+  apply PTree.extensionality;
+  intros i;
+  rewrite PTree.gsspec;
+  rewrite PTree.gmap1;
+  rewrite PTree.gsspec;
+  destruct (Coqlib.peq i _);
+  try subst; try reflexivity;
+  try rewrite PTree.gmap1; try reflexivity.
+
+Ltac prove_lookup_varlike_after_update_all_varlike :=
+  intros T s1 v fv;
+  unfold new_pmap_from_old, PMap.get;
+  simpl;
+  destruct v eqn:des;
+  rewrite PTree.gmap;
+  unfold Coqlib.option_map;
+  lazymatch goal with
+  | |- context[match match ?e with _ => _ end with _ => _ end] =>
+      let He := fresh "He" in destruct e eqn:He
+  end; congruence.
+
 Instance CrVarLike_Header : CrVarLike Header.
 Proof.
   refine {| make_item := fun uid => HeaderCtr uid;
             get_key := fun h => match h with HeaderCtr uid => uid end;
-            inverses := _;
-            inj := _ |}.
+            map_from_ps := fun (T : Type) (ps : ProgramState T) => header_map ps;
+            update_all_varlike := fun (T : Type) (ps : ProgramState T) (fh : Header -> T) =>
+              let new_map := new_pmap_from_old (header_map ps) (fun pos => fh (HeaderCtr pos)) in
+              {| ctrl_map := ctrl_map ps;
+                 header_map := new_map;
+                 state_map := state_map ps |};
+            update_varlike := fun (T : Type) (ps : ProgramState T) (h : Header) (v : T) =>
+              let new_map := PMap.set (match h with HeaderCtr uid => uid end) v (header_map ps) in
+              {| ctrl_map := ctrl_map ps;
+                 header_map := new_map;
+                 state_map := state_map ps |}; |}.
   - (* inverses : forall x, make_item (get_key x) = x *)
     intros [uid]. simpl. reflexivity.
   - (* inverses' : forall i, get_key (make_item i) = i *)
     reflexivity.
   - (* inj : injective_contravariant get_key *)
     prove_inj.
+  - (* update_all_varlike_lookup_unchanged : forall {T} (s1 : ProgramState T), update_all_varlike s1 (fun v : A => lookup_varlike_map (map_from_ps s1) v) = s1; *)
+    prove_update_all_varlike_lookup_unchanged hdr.
+  - (* commute_lookup_varlike:
+      forall {T1 T2} (ps : ProgramState T1) (v : A) (func : T1 -> T2), lookup_varlike (program_state_mapper func func func ps) v = func (lookup_varlike_map (map_from_ps ps) v); *)
+    intros. apply PMap.gmap.
+  - (* commute_mapper_update_varlike:
+      forall {T1 T2} (ps : ProgramState T1) (x : A) (v : T1) (func : T1 -> T2),
+      program_state_mapper func func func (update_varlike ps x v) = update_varlike (program_state_mapper func func func ps) x (func v) *)
+    prove_commute_mapper_update_varlike.
+  - (* lookup_varlike_after_update_all_varlike:
+      forall {T} (s1 : ProgramState T) (v : A) (fv : A -> T),
+        is_varlike_in_ps s1 v <> None ->
+        lookup_varlike_map (map_from_ps (update_all_varlike s1 fv)) v = fv v; *)
+    prove_lookup_varlike_after_update_all_varlike.
 Defined.
 
 Instance CrVarLike_State : CrVarLike State.
 Proof.
   refine {| make_item := fun uid => StateCtr uid;
             get_key := fun s => match s with StateCtr uid => uid end;
-            inverses := _;
-            inj := _ |}.
+            map_from_ps := fun (T : Type) (ps : ProgramState T) => state_map ps;
+            update_all_varlike := fun (T : Type) (ps : ProgramState T) (fs : State -> T) =>
+              let new_map := new_pmap_from_old (state_map ps) (fun pos => fs (StateCtr pos)) in
+              {| ctrl_map := ctrl_map ps;
+                 header_map := header_map ps;
+                 state_map := new_map |};
+            update_varlike := fun (T : Type) (ps : ProgramState T) (h : State) (v : T) =>
+              let new_map := PMap.set (match h with StateCtr uid => uid end) v (state_map ps) in
+              {| ctrl_map := ctrl_map ps;
+                 header_map := header_map ps;
+                 state_map := new_map |}; |}.
   - intros [uid]. simpl. reflexivity.
   - reflexivity.
   - prove_inj.
+  - prove_update_all_varlike_lookup_unchanged state.
+  - intros. apply PMap.gmap.
+  - prove_commute_mapper_update_varlike.
+  - prove_lookup_varlike_after_update_all_varlike.
 Defined.
 
 Instance CrVarLike_Ctrl : CrVarLike Ctrl.
 Proof.
   refine {| make_item := fun uid => CtrlCtr uid;
             get_key := fun s => match s with CtrlCtr uid => uid end;
-            inverses := _;
-            inj := _ |}.
+            map_from_ps := fun (T : Type) (ps : ProgramState T) => ctrl_map ps;
+            update_all_varlike := fun (T : Type) (ps : ProgramState T) (fs : Ctrl -> T) =>
+              let new_map := new_pmap_from_old (ctrl_map ps) (fun pos => fs (CtrlCtr pos)) in
+              {| ctrl_map := new_map;
+                 header_map := header_map ps;
+                 state_map := state_map ps |};
+            update_varlike := fun (T : Type) (ps : ProgramState T) (h : Ctrl) (v : T) =>
+              let new_map := PMap.set (match h with CtrlCtr uid => uid end) v (ctrl_map ps) in
+              {| ctrl_map := new_map;
+                 header_map := header_map ps;
+                 state_map := state_map ps |}; |}.
   - intros [uid]. simpl. reflexivity.
   - reflexivity.
   - prove_inj.
+  - prove_update_all_varlike_lookup_unchanged ctrl.
+  - intros. apply PMap.gmap.
+  - prove_commute_mapper_update_varlike.
+  - prove_lookup_varlike_after_update_all_varlike.
 Defined.
 
 Section CrVarLikeEqual.
@@ -110,3 +256,134 @@ Proof.
 Qed.
 
 End CrVarLikeEqual.
+
+Instance CrVarLikePairLemmas_Header_State : CrVarLikePairLemmas Header State CrVarLike_Header CrVarLike_State.
+Proof.
+  refine {| test := HeaderCtr xH;|}.
+  - intros.
+    simpl.
+    f_equal.
+Defined.
+
+Instance CrVarLikePairLemmas_State_Header : CrVarLikePairLemmas State Header CrVarLike_State CrVarLike_Header.
+Proof.
+  refine {| test := StateCtr xH;|}.
+  - intros.
+    simpl.
+    f_equal.
+Defined.
+
+Lemma program_state_equality:
+      forall (ps1 ps2: ConcreteState),
+        ctrl_map ps1 = ctrl_map ps2 ->
+        header_map ps1 = header_map ps2 ->
+        state_map  ps1 = state_map ps2 ->
+        ps1 = ps2.
+Proof.
+  intros ps1 ps2 Hctrl Hhdr Hstate.
+  destruct ps1 as [ctrl1 hdr1 state1].
+  destruct ps2 as [ctrl2 hdr2 state2].
+  simpl in *.
+  f_equal; try assumption.
+Qed.
+
+Lemma program_state_unchanged:
+  forall {T} (s1 : ProgramState T),
+  update_all_varlike (update_all_varlike s1 (fun h : Header => lookup_varlike_map (map_from_ps s1) h))
+                    (fun s : State => lookup_varlike_map (map_from_ps s1) s) = s1.
+Admitted.
+
+(* TODO: Does this hold if A = A'? Similar to lemma before. *)
+Lemma is_v1_in_ps_after_update_all_v2:
+  forall {T A A'} `{CrVarLike A} `{CrVarLike A'} (s1 : ProgramState T)
+    (h : A) (fs : A' -> T),
+    is_varlike_in_ps (update_all_varlike s1 fs) h = is_varlike_in_ps s1 h.
+Admitted.
+(*
+Proof.
+  intros.
+  destruct f1, f2; try congruence;
+  reflexivity.
+Qed.
+*)
+
+Definition get_all_varlike_from_ps {T A : Type} `{CrVarLike A} (s: ProgramState T) : list A :=
+  List.map (fun '(key, value) => make_item key)
+           (PTree.elements (snd (map_from_ps s))).
+
+Lemma is_varlike_in_ps_lemma :
+  forall {T A} `{CrVarLike A} (s1 : ProgramState T) (v : A),
+    In v (get_all_varlike_from_ps s1) ->
+    is_varlike_in_ps s1 v <> None.
+Admitted.
+(*
+Proof.
+  intros T A HA f s1 v H.
+  destruct s1 as [ctrl hdr state].
+  destruct f;
+  unfold get_all_varlike_from_ps in H;
+  unfold is_varlike_in_ps;
+  simpl in *;
+  destruct ctrl as [c0 ctrl_map];
+  destruct hdr as [h0 hdr_map];
+  destruct state as [s0 state_map];
+  simpl in *;
+  apply in_map_iff in H;
+  destruct H; (* TODO: ask Joe, seems to extract witness *)
+  destruct x;
+  destruct H;
+  rewrite <- H; rewrite inverses';
+  apply some_is_not_none with (x := t);
+  apply PTree.elements_complete;
+  assumption.
+Qed.
+*)
+
+Definition init_concrete_state (p : CaracaraProgram) : ConcreteState :=
+  let h := get_headers_from_prog p in
+  let s := get_states_from_prog p in
+  let c := get_ctrls_from_prog p in
+  {|ctrl_map    :=  (repr 0, (* TODO: Need better default, but think this doesn't matter *)
+                    PTree_Properties.of_list
+                    (List.map (fun x => (match x with | CtrlCtr x_id => x_id end, repr 0)) c));
+     header_map :=  (repr 0, (* TODO: Need better default, but think this doesn't matter *)
+                    PTree_Properties.of_list
+                    (List.map (fun x => (match x with | HeaderCtr x_id => x_id end, repr 0)) h));
+     state_map  :=  (repr 0,
+                    PTree_Properties.of_list
+                    (List.map (fun x => (match x with | StateCtr x_id => x_id end, repr 0)) s));|}.
+
+(* Convert positive to string *)
+Fixpoint pos_to_string (p : positive) : string :=
+  match p with
+  | xH => "1"
+  | xO p' => String.append (pos_to_string p') "0"
+  | xI p' => String.append (pos_to_string p') "1"
+  end.
+
+Definition init_symbolic_state (p: CaracaraProgram) : SymbolicState :=
+  let h := get_headers_from_prog p in
+  let s := get_states_from_prog p in
+  let c := get_ctrls_from_prog p in
+  {|ctrl_map :=  (SmtArithVar "rndstring", (*TODO: Need better default, but think this doesn't matter *)
+                        PTree_Properties.of_list
+                        (List.map (fun x => let var := match x with | CtrlCtr x_id => x_id end in (var,  SmtArithVar (pos_to_string var))) c));
+     header_map     :=  (SmtArithVar "rndstring", (*TODO: Need better default, but think this doesn't matter *)
+                        PTree_Properties.of_list
+                        (List.map (fun x => let var := match x with | HeaderCtr x_id => x_id end in (var, SmtArithVar (pos_to_string var))) h));
+     state_map  :=  (SmtArithVar "rndstring", (*TODO: Need better default, but think this doesn't matter *)
+                        PTree_Properties.of_list
+                        (List.map (fun x => let var := match x with | StateCtr x_id => x_id end in (var, SmtArithVar (pos_to_string var))) s));|}.
+
+Definition is_init_state {T} (p : CaracaraProgram) (ps : ProgramState T) : Prop :=
+  forall h sv c,
+    (In h (get_headers_from_prog p) <-> In h (get_all_varlike_from_ps ps)) /\
+    (In sv (get_states_from_prog p) <-> In sv (get_all_varlike_from_ps ps)) /\
+    (In c (get_ctrls_from_prog p) <-> In c (get_all_varlike_from_ps ps)).
+
+(* Mark definitions globally opaque below *)
+Global Opaque lookup_varlike_map.
+Global Opaque program_state_mapper.
+Global Opaque new_pmap_from_old.
+Global Opaque get_all_varlike_from_ps.
+Global Opaque map_from_ps.
