CrDsl.v
@@ -6,7 +6,6 @@ Require Import List.
 Import ListNotations.
 Require Import Strings.String.
 From MyProject Require Import CrIdentifiers.
-From MyProject Require Import CrVarLike.
 From MyProject Require Import CrParser.
 From MyProject Require Import CrTransformer.
 From MyProject Require Import ListUtils.
@@ -53,35 +52,3 @@ Definition get_transformer_from_prog (p : CaracaraProgram) : Transformer :=
   match p with
   | CaracaraProgramDef _ _ _ t => t
   end.
-
-(* Check for duplicate identifiers in the header, state, and control lists *)
-Definition check_for_duplicate_identifiers (program : CaracaraProgram) : bool :=
-  match program with
-  | CaracaraProgramDef h s c _ =>
-      (* TODO: can probably adjust has_duplicates *)
-      has_duplicates varlike_equal h ||
-      has_duplicates varlike_equal s ||
-      has_duplicates varlike_equal c
-  end.
-
-From Coq Require Import Sorting.Sorted.
-Check Sorted.
-
-(* Compare two headers based on their uids *)
-Section VarlikeCmp.
-Context {A : Type} {CrVarLike_A : CrVarLike A}.
-Definition varlike_lt (v1 v2: A) : Prop :=
-  Pos.lt (get_key v1) (get_key v2).
-End VarlikeCmp.
-
-(* No duplicates in Caracara Program *)
-Definition well_formed_program (p : CaracaraProgram) : Prop :=
-  match p with
-  | CaracaraProgramDef h s c _ =>
-      Coqlib.list_norepet h /\ Coqlib.list_norepet s /\ Coqlib.list_norepet c /\
-      Sorted varlike_lt h /\ Sorted varlike_lt s /\ Sorted varlike_lt c
-  end.
-
-(* TODO: Write a program to check for the well_formed_program property *)
-(* TODO: This would involve checking for duplicates and sorting the lists *)
-(* TODO: And then verifying the well_formed_program property holds *)
