HelperLemmas.v
@@ -14,29 +14,18 @@ From MyProject Require Import CrProgramState.
 From MyProject Require Import ListUtils.
 
 Lemma commute_lookup_eval_varlike:
-  forall {A} `{CrVarLike A} (field : PSField) (ps : SymbolicState)
+  forall {A} `{CrVarLike A} (ps : SymbolicState)
         (var : A) (val : SmtValuation),
-    lookup_varlike field (eval_sym_state ps val) var =
-    eval_smt_arith (lookup_varlike field ps var) val.
-Proof.
-  intros.
-  destruct field;
-  unfold eval_sym_state;
-  rewrite commute_lookup_varlike;
-  reflexivity.
-Qed.
+    lookup_varlike (eval_sym_state ps val) var =
+    eval_smt_arith (lookup_varlike ps var) val.
+Admitted.
 
 Lemma commute_lookup_eval:
   forall (s : SymbolicState) (f : SmtValuation)
         arg,
     lookup_concrete arg (eval_sym_state s f) =
     eval_smt_arith (lookup_smt arg s) f.
-Proof.
-  intros s f arg.
-  unfold lookup_concrete.
-  destruct arg; simpl; try reflexivity;
-  apply commute_lookup_eval_varlike.
-Qed.
+Admitted.
 
 Lemma find_first_match_lemma:
   forall {T : Set} (list_of_pair :  list (bool*T)),
